lunarlander_sl/BigStepContinuous.thy
@@ -8,6 +8,9 @@ subsection \<open>Hoare rules for ODE\<close>
 inductive_cases contE: "big_step (Cont ode b) s1 tr s2"
 thm contE
 
+inductive_cases interruptE: "big_step (Interrupt ode cs) s1 tr s2"
+thm interruptE
+
 text \<open>Weakest precondition form\<close>
 theorem Valid_ode:
   "Valid
@@ -23,15 +26,15 @@ text \<open>Strongest postcondition form\<close>
 theorem Valid_ode':
   assumes "b st"
   shows "Valid
-    (\<lambda>s tr. s = st \<and> tr = [])
+    (\<lambda>s t. s = st \<and> t = tr)
     (Cont ode b)
-    (\<lambda>s tr. (\<exists>d p. 0 < d \<and> ODEsol ode p d \<and> p 0 = st \<and> (\<forall>t. 0 \<le> t \<and> t < d \<longrightarrow> b (p t)) \<and> \<not>b (p d) \<and>
-                   s = p d \<and> tr = [WaitBlock d (\<lambda>\<tau>\<in>{0..d}. State (p \<tau>)) ({}, {})]))"
+    (\<lambda>s t. (\<exists>d p. 0 < d \<and> ODEsol ode p d \<and> p 0 = st \<and> (\<forall>t. 0 \<le> t \<and> t < d \<longrightarrow> b (p t)) \<and> \<not>b (p d) \<and>
+                   s = p d \<and> t = tr @ [WaitBlock d (\<lambda>\<tau>\<in>{0..d}. State (p \<tau>)) ({}, {})]))"
   apply (rule Valid_weaken_pre)
   prefer 2 apply (rule Valid_ode)
   by (auto simp add: entails_def assms)
 
-
+text \<open>Unique solution form\<close>
 theorem Valid_ode_unique_solution:
   assumes
     "d > 0" "ODEsol ode p d" "\<forall>t. t \<ge> 0 \<and> t < d \<longrightarrow> b (p t)"
@@ -109,6 +112,122 @@ proof -
       using main[of d1 p1] by auto
     done
 qed
+
+
+subsection \<open>Hoare rules for ODE\<close>
+
+text \<open>Weakest precondition form\<close>
+theorem Valid_interrupt:
+  assumes "\<forall>i<length cs.
+    case cs ! i of
+      (ch[!]e, p2) \<Rightarrow>
+        (\<exists>Q. Valid Q p2 R \<and>
+             (P \<Longrightarrow>\<^sub>A (\<lambda>s tr. Q s (tr @ [OutBlock ch (e s)]))) \<and>
+             (P \<Longrightarrow>\<^sub>A (\<lambda>s tr. \<forall>d>0. \<forall>p. ODEsol ode p d \<longrightarrow> p 0 = s \<longrightarrow>
+                        Q (p d) (tr @ [WaitBlock d (\<lambda>\<tau>\<in>{0..d}. State (p \<tau>)) (rdy_of_echoice cs),
+                                       OutBlock ch (e (p d))]))))
+    | (ch[?]var, p2) \<Rightarrow>
+        (\<exists>Q. Valid Q p2 R \<and>
+             (P \<Longrightarrow>\<^sub>A (\<lambda>s tr. \<forall>v. Q (s(var := v)) (tr @ [InBlock ch v]))) \<and>
+             (P \<Longrightarrow>\<^sub>A (\<lambda>s tr. \<forall>d>0. \<forall>p v. ODEsol ode p d \<longrightarrow> p 0 = s \<longrightarrow>
+                        Q ((p d)(var := v)) (tr @ [WaitBlock d (\<lambda>\<tau>\<in>{0..d}. State (p \<tau>)) (rdy_of_echoice cs),
+                                                   InBlock ch v]))))"
+  shows "Valid P (Interrupt ode cs) R"
+proof -
+  have a: "R s2 (tr1 @ OutBlock ch (e s1) # tr2)"
+    if *: "P s1 tr1"
+          "i < length cs"
+          "cs ! i = (ch[!]e, p2)"
+          "big_step p2 s1 tr2 s2" for s1 tr1 s2 i ch e p2 tr2
+  proof -
+    from assms obtain Q where 1:
+      "Valid Q p2 R"
+      "P \<Longrightarrow>\<^sub>A (\<lambda>s tr. Q s (tr @ [OutBlock ch (e s)]))"
+      using *(2,3) by fastforce
+    have 2: "Q s1 (tr1 @ [OutBlock ch (e s1)])"
+      using 1(2) *(1) unfolding entails_def by auto
+    then show ?thesis
+      using *(4) 1(1) unfolding Valid_def by fastforce
+  qed
+  have b: "R s2 (tr1 @ WaitBlock d (\<lambda>\<tau>\<in>{0..d}. State (p \<tau>)) (rdy_of_echoice cs) # OutBlock ch (e (p d)) # tr2)"
+    if *: "P (p 0) tr1"
+          "0 < d"
+          "ODEsol ode p d"
+          "i < length cs"
+          "cs ! i = (ch[!]e, p2)"
+          "big_step p2 (p d) tr2 s2" for tr1 s2 d p i ch e p2 tr2
+  proof -
+    from assms obtain Q where 1:
+      "Valid Q p2 R"
+      "P \<Longrightarrow>\<^sub>A (\<lambda>s tr. \<forall>d>0. \<forall>p. ODEsol ode p d \<longrightarrow> p 0 = s \<longrightarrow>
+                 Q (p d) (tr @ [WaitBlock d (\<lambda>\<tau>\<in>{0..d}. State (p \<tau>)) (rdy_of_echoice cs),
+                                OutBlock ch (e (p d))]))"
+      using *(4,5) by fastforce
+    have "Q (p d) (tr1 @ [WaitBlock d (\<lambda>\<tau>\<in>{0..d}. State (p \<tau>)) (rdy_of_echoice cs),
+                          OutBlock ch (e (p d))])"
+      using 1(2) *(1-3) unfolding entails_def by auto
+    then show ?thesis
+      using *(6) 1(1) unfolding Valid_def by fastforce
+  qed
+  have c: "R s2 (tr1 @ InBlock ch v # tr2)"
+    if *: "P s1 tr1"
+          "i < length cs"
+          "cs ! i = (ch[?]var, p2)"
+          "big_step p2 (s1(var := v)) tr2 s2" for s1 tr1 s2 i ch var p2 v tr2
+  proof -
+    from assms obtain Q where 1:
+      "Valid Q p2 R"
+      "P \<Longrightarrow>\<^sub>A (\<lambda>s tr. \<forall>v. Q (s(var := v)) (tr @ [InBlock ch v]))"
+      using *(2,3) by fastforce
+    have 2: "Q (s1(var := v)) (tr1 @ [InBlock ch v])"
+      using 1(2) *(1) unfolding entails_def by auto
+    then show ?thesis
+      using *(4) 1(1) unfolding Valid_def by fastforce
+  qed
+  have d: "R s2 (tr1 @ WaitBlock d (\<lambda>\<tau>\<in>{0..d}. State (p \<tau>)) (rdy_of_echoice cs) # InBlock ch v # tr2a)"
+    if *: "P (p 0) tr1"
+          "0 < d"
+          "ODEsol ode p d"
+          "i < length cs"
+          "cs ! i = (ch[?]var, p2)"
+          "big_step p2 ((p d)(var := v)) tr2a s2" for tr1 s2 d p i ch var p2 v tr2a
+  proof -
+    from assms obtain Q where 1:
+      "Valid Q p2 R"
+      "P \<Longrightarrow>\<^sub>A (\<lambda>s tr. \<forall>d>0. \<forall>p v. ODEsol ode p d \<longrightarrow> p 0 = s \<longrightarrow>
+                 Q ((p d)(var := v)) (tr @ [WaitBlock d (\<lambda>\<tau>\<in>{0..d}. State (p \<tau>)) (rdy_of_echoice cs),
+                                            InBlock ch v]))"
+      using *(4,5) by fastforce
+    have "Q ((p d)(var := v)) (tr1 @ [WaitBlock d (\<lambda>\<tau>\<in>{0..d}. State (p \<tau>)) (rdy_of_echoice cs), InBlock ch v])"
+      using 1(2) *(1-3) unfolding entails_def by auto
+    then show ?thesis
+      using *(6) 1(1) unfolding Valid_def by fastforce
+  qed
+  show ?thesis
+    unfolding Valid_def
+    apply (auto elim!: interruptE) using a b c d by auto
+qed
+
+theorem Valid_interrupt_InIn:
+  assumes "Valid Q1 p1 R"
+    and "Valid Q2 p2 R"
+  shows "Valid
+    (\<lambda>s tr. (\<forall>v. Q1 (s(var1 := v)) (tr @ [InBlock ch1 v])) \<and>
+            (\<forall>d>0. \<forall>p v. ODEsol ode p d \<longrightarrow> p 0 = s \<longrightarrow>
+                Q1 ((p d)(var1 := v)) (tr @ [WaitBlock d (\<lambda>\<tau>\<in>{0..d}. State (p \<tau>)) ({}, {ch1, ch2}),
+                                             InBlock ch1 v])) \<and>
+            (\<forall>v. Q2 (s(var2 := v)) (tr @ [InBlock ch2 v])) \<and>
+            (\<forall>d>0. \<forall>p v. ODEsol ode p d \<longrightarrow> p 0 = s \<longrightarrow>
+                Q2 ((p d)(var2 := v)) (tr @ [WaitBlock d (\<lambda>\<tau>\<in>{0..d}. State (p \<tau>)) ({}, {ch1, ch2}),
+                                             InBlock ch2 v])))
+      (Interrupt ode [(ch1[?]var1, p1), (ch2[?]var2, p2)])
+    R"
+  apply (rule Valid_interrupt)
+  apply (rule InIn_lemma)
+  subgoal apply (rule exI[where x=Q1])
+    by (auto simp add: assms entails_def)
+  apply (rule exI[where x=Q2])
+  by (auto simp add: assms entails_def)
 
 
 subsection \<open>Tests for ODE\<close>
